LambdaS5/coq/Monads.v
@@ -16,31 +16,31 @@ Implicit Type store : Store.store.
 
 (* Evaluate an expression, and calls the continuation with
 * the new store and the Context.result of the evaluation. *)
-Definition eval_cont {value_type : Type} runs store (e : Syntax.expression) (cont : Store.store -> (@Context.result Values.value_loc) -> (Store.store * (@Context.result value_type))) : (Store.store * (@Context.result value_type)) :=
+Definition eval_cont {value_type : Type} runs store (e : Syntax.expression) (cont : Store.store -> (Context.result Values.value_loc) -> (Store.store * (Context.result value_type))) : (Store.store * (Context.result value_type)) :=
   match ((Context.runs_type_eval runs) store e) with (store, res) =>
     cont store res
   end
 .
 (* Alias for calling eval_cont with an empty continuation *)
-Definition eval_cont_terminate runs store (e : Syntax.expression) : (Store.store * Context.result) :=
+Definition eval_cont_terminate runs store (e : Syntax.expression) : (Store.store * Context.result Values.value_loc) :=
   eval_cont runs store e (fun store res => (store, res))
 .
 
 (* Calls the continuation if the variable is a value.
 * Returns the variable and the store verbatim otherwise. *)
-Definition if_return {value_type : Type} {value_type_2 : Type} store (var : @Context.result value_type) (cont : value_type -> (Store.store * (@Context.result value_type_2))) : (Store.store * (@Context.result value_type_2)) :=
+Definition if_return {value_type : Type} {return_type : Type} store (var : Context.result value_type) (cont : value_type -> (Store.store * (Context.result return_type))) : (Store.store * (Context.result return_type)) :=
   match var with
   | Return v => cont v
-  | Exception exc => (store, Exception exc)
-  | Break b v => (store, Break b v)
-  | Fail f => (store, Fail f)
+  | Exception exc => (store, Exception return_type exc)
+  | Break b v => (store, Break return_type b v)
+  | Fail f => (store, Fail return_type f)
   end
 .
 
 (* Evaluates an expression, and calls the continuation if
 * the evaluation returned a value.
 * Returns the store and the variable verbatim otherwise. *)
-Definition if_eval_return {value_type : Type} runs store (e : Syntax.expression) (cont : Store.store -> Values.value_loc -> (Store.store * (@Context.result value_type))) : (Store.store * (@Context.result value_type)) :=
+Definition if_eval_return {value_type : Type} runs store (e : Syntax.expression) (cont : Store.store -> Values.value_loc -> (Store.store * (Context.result value_type))) : (Store.store * (Context.result value_type)) :=
   eval_cont runs store e (fun store res =>
     if_return store res (cont store)
   )
@@ -49,7 +49,7 @@ Definition if_eval_return {value_type : Type} runs store (e : Syntax.expression)
 (* Evaluates an expression with if it is Some, and calls the continuation
 * if the evaluation returned value. Calls the continuation with the default
 * value if the expression is None. *)
-Definition if_some_eval_else_default {value_type : Type} runs store (oe : option Syntax.expression) (default : Values.value_loc) (cont : Store.store -> Values.value_loc -> (Store.store * (@Context.result value_type))) : (Store.store * (@Context.result value_type)) :=
+Definition if_some_eval_else_default {value_type : Type} runs store (oe : option Syntax.expression) (default : Values.value_loc) (cont : Store.store -> Values.value_loc -> (Store.store * (Context.result value_type))) : (Store.store * (Context.result value_type)) :=
   match oe with
   | Some e => if_eval_return runs store e cont
   | None => cont store default
@@ -58,7 +58,7 @@ Definition if_some_eval_else_default {value_type : Type} runs store (oe : option
 
 (* Same as if_some_and_eval_value, but returns an option as the Context.result, and
 * None is used as the default value passed to the continuation. *)
-Definition if_some_eval_return_else_none {value_type : Type} runs store (oe : option Syntax.expression) (cont : Store.store -> option Values.value_loc -> (Store.store * (@Context.result value_type))) : (Store.store * (@Context.result value_type)) :=
+Definition if_some_eval_return_else_none {value_type : Type} runs store (oe : option Syntax.expression) (cont : Store.store -> option Values.value_loc -> (Store.store * (Context.result value_type))) : (Store.store * (Context.result value_type)) :=
   match oe with
   | Some e => if_eval_return runs store e (fun ctx res => cont ctx (Some res))
   | None => cont store None
@@ -67,41 +67,41 @@ Definition if_some_eval_return_else_none {value_type : Type} runs store (oe : op
 
 (* Calls the continuation with the referenced value. Fails if the reference
 * points to a non-existing object (never actually happens). *)
-Definition assert_deref {value_type : Type} store (loc : Values.value_loc) (cont : Values.value -> (Store.store * (@Context.result value_type))) : (Store.store * (@Context.result value_type)) :=
+Definition assert_deref {value_type : Type} store (loc : Values.value_loc) (cont : Values.value -> (Store.store * (Context.result value_type))) : (Store.store * (Context.result value_type)) :=
   match (Store.get_value store loc) with
   | Some val => cont val
-  | None => (store, Fail "Location of non-existing value.")
+  | None => (store, Fail value_type "Location of non-existing value.")
   end
 .
 
 (* Calls the continuation if the value is a location to a value (always!), and passes the value to the continuation.
 * Fails otherwise. *)
-Definition assert_get {value_type : Type} store (loc : Values.value_loc) (cont : Values.value -> (Store.store * (@Context.result value_type))) : (Store.store * (@Context.result value_type)) :=
+Definition assert_get {value_type : Type} store (loc : Values.value_loc) (cont : Values.value -> (Store.store * (Context.result value_type))) : (Store.store * (Context.result value_type)) :=
   match (Store.get_value store loc) with
   | Some val => cont val
-  | None => (store, Fail "Location of non-existing value.")
+  | None => (store, Fail value_type "Location of non-existing value.")
   end
 .
 
 (* Calls the continuation if the value is an object pointer, and passes the pointer to the continuation.
 * Fails otherwise. *)
-Definition assert_get_object_ptr {value_type : Type} store (loc : Values.value_loc) (cont : Values.object_ptr -> (Store.store * (@Context.result value_type))) : (Store.store * (@Context.result value_type)) :=
+Definition assert_get_object_ptr {value_type : Type} store (loc : Values.value_loc) (cont : Values.object_ptr -> (Store.store * (Context.result value_type))) : (Store.store * (Context.result value_type)) :=
   match (Store.get_value store loc) with
   | Some (Values.Object ptr) => cont ptr
-  | Some _ => (store, Fail "Expected an object pointer.")
-  | None => (store, Fail "Location of non-existing value.")
+  | Some _ => (store, Fail value_type "Expected an object pointer.")
+  | None => (store, Fail value_type "Location of non-existing value.")
   end
 .
 
-Definition assert_get_object_from_ptr {value_type : Type} store (ptr : Values.object_ptr) (cont : Values.object -> (Store.store * (@Context.result value_type))) : (Store.store * (@Context.result value_type)) :=
+Definition assert_get_object_from_ptr {value_type : Type} store (ptr : Values.object_ptr) (cont : Values.object -> (Store.store * (Context.result value_type))) : (Store.store * (Context.result value_type)) :=
   match (Store.get_object store ptr) with
   | Some obj => cont obj
-  | None => (store, Fail "Pointer to a non-existing object.")
+  | None => (store, Fail value_type "Pointer to a non-existing object.")
   end
 .
 
 (* Calls the continuation if the value is an object pointer, and passes the object to the continuation *)
-Definition assert_get_object {value_type : Type} store (loc : Values.value_loc) (cont : Values.object -> (Store.store * (@Context.result value_type))) : (Store.store * (@Context.result value_type)) :=
+Definition assert_get_object {value_type : Type} store (loc : Values.value_loc) (cont : Values.object -> (Store.store * (Context.result value_type))) : (Store.store * (Context.result value_type)) :=
   assert_get_object_ptr store loc (fun ptr =>
     assert_get_object_from_ptr store ptr cont
   )
@@ -109,22 +109,22 @@ Definition assert_get_object {value_type : Type} store (loc : Values.value_loc) 
 
 (* Calls the continuation if the value is a string.
 * Fails otherwise. *)
-Definition assert_get_string {value_type : Type} store (loc : Values.value_loc) (cont : string -> (Store.store * (@Context.result value_type))) : (Store.store * (@Context.result value_type)) :=
+Definition assert_get_string {value_type : Type} store (loc : Values.value_loc) (cont : string -> (Store.store * (Context.result value_type))) : (Store.store * (Context.result value_type)) :=
   match (Store.get_value store loc) with
   | Some (Values.String s) => cont s
-  | Some _ => (store, Fail "Expected String but did not get one.")
-  | None => (store, Fail "Location of non-existing value.")
+  | Some _ => (store, Fail value_type "Expected String but did not get one.")
+  | None => (store, Fail value_type "Location of non-existing value.")
   end
 .
 
 (* Calls the continuation if the value is a boolean.
 * Fails otherwise. *)
-Definition assert_get_bool_3 {value_type : Type} {X : Type} store (loc : Values.value_loc) (default : X) (cont : bool -> (Store.store * X * (@Context.result value_type))) : (Store.store * X * (@Context.result value_type)) :=
+Definition assert_get_bool_3 {value_type : Type} {X : Type} store (loc : Values.value_loc) (default : X) (cont : bool -> (Store.store * X * (Context.result value_type))) : (Store.store * X * (Context.result value_type)) :=
   match (Store.get_value store loc) with
   | Some Values.True => cont true
   | Some Values.False => cont false
-  | Some _ => (store, default, Fail "Expected True or False but got none of them.")
-  | None => (store, default, Fail "Location of non-existing value.")
+  | Some _ => (store, default, Fail value_type "Expected True or False but got none of them.")
+  | None => (store, default, Fail value_type "Location of non-existing value.")
   end
 .
 
